array: finish sequential proof

array-contains.bpl
@@ -1,22 +1,59 @@
 // A simplified hash table implementation with weakly consistent contains method
 
-type Invoc;
 
-type SeqInvoc;  // sequence of invocations
+// ---------- Encoding of weak visibility
+
+type Invoc;
 
 // Create an invocation. Methods are: 0 - put, 1 - get, 2 - contains
 function createInvoc(m: int, k: int, v: int) returns (i: Invoc);
 
-function append(s: SeqInvoc, i: Invoc) returns (t: SeqInvoc);
 
-// A function to calculate the abstract state after a sequential execution
-function state(s: SeqInvoc) returns (m: [int]int);
+type SeqInvoc;  // sequence of invocations
+
+
+function subseq(s: SeqInvoc, t: SeqInvoc) : bool;
+
+// subseq is reflexive
+axiom (forall s: SeqInvoc :: subseq(s, s));
+
+// subseq is transitive
+axiom (forall s, t, u: SeqInvoc :: subseq(s, t) && subseq(t, u) ==> subseq(s, u));
+
+
+function append(s: SeqInvoc, o: Invoc) returns (t: SeqInvoc);
+
+// append preserves subseq
+axiom (forall s, t: SeqInvoc, o: Invoc :: subseq(s, t) ==> subseq(append(s, o), append(t, o)));
+
+
+function union(s1: SeqInvoc, s2: SeqInvoc) returns (t: SeqInvoc);
+
+// union is idempotent
+axiom (forall s: SeqInvoc :: s == union(s, s));
+
+// union is associative
+axiom (forall s, t: SeqInvoc :: union(s, t) == union(t, s));
+
+// union is monotonic w.r.t subseq
+axiom (forall s, t1, t2: SeqInvoc :: subseq(t1, t2) ==> subseq(union(s, t1), union(s, t2)));
+
 
 // A function to restrict a SeqInvoc to invocations involving key k
 function restr(s: SeqInvoc, k: int) returns (t: SeqInvoc);
 
+// restr is a subseq
+axiom (forall s: SeqInvoc, k: int :: subseq(restr(s, k), s));
+
+
+// A function to calculate the abstract state after a sequential execution
+function state(s: SeqInvoc) returns (m: [int]int);
+
 // The mapping of key k depends only invocations involving k
 axiom (forall s: SeqInvoc, k: int :: state(s)[k] == state(restr(s, k))[k]);
+
+// Adding invocations of a key k does not affect state of keys k1 != k
+axiom (forall s, t: SeqInvoc, k, k1: int :: k != k1 ==> state(union(s, restr(t, k)))[k1] == state(s)[k1]);
 
 
 // ---------- Some lemmas that we need
@@ -25,6 +62,14 @@ procedure lemma_append_effect(s1, s2: SeqInvoc, o: Invoc, m, k, v: int)
   requires s2 == append(s1, o) && o == createInvoc(m, k, v);
   ensures (forall i: int :: i != k ==> state(s1)[i] == state(s2)[i]);
   ensures m == 0 ==> state(s2)[k] == v;
+  ensures m == 1 || m == 2 ==> state(s2)[k] == state(s1)[k];
+{
+  assume false;
+}
+
+procedure lemma_union_restr(s0, s1, t: SeqInvoc, k: int)
+  requires s1 == union(s0, restr(t, k)) && subseq(s0, t);
+  ensures restr(s1, k) == restr(t, k);
 {
   assume false;
 }
@@ -37,7 +82,8 @@ var lin: SeqInvoc;  // a shared global variable that builds the linearization
 
 // Concrete state of implementation
 var table: [int]int;
-var tableLen: int;
+const tableLen: int;
+axiom 0 <= tableLen;
 
 
 // ---------- Procedures/methods
@@ -60,13 +106,81 @@ procedure put(k: int, v: int)
 }
 
 procedure get(k: int) returns (v: int)
+  modifies lin;
   requires 0 <= k && k < tableLen;
   requires (forall i: int :: 0 <= i && i < tableLen ==> table[i] == state(lin)[i]);
   ensures (forall i: int :: 0 <= i && i < tableLen ==> table[i] == state(lin)[i]);
 {
+  var old_lin: SeqInvoc;
+  var invoc: Invoc;
   v := table[k];
 
-  assert state(lin)[k] == v;
-  lin := append(lin, this);
-  return v;
+  old_lin := lin;
+  invoc := createInvoc(1, k, v);
+  lin := append(lin, invoc);
+  call lemma_append_effect(old_lin, lin, invoc, 1, k, v);
+}
+
+procedure contains(v: int) returns (res: bool, vis: SeqInvoc, witness_k: int)
+  modifies lin;
+  requires (forall i: int :: 0 <= i && i < tableLen ==> table[i] == state(lin)[i]);
+  ensures (forall i: int :: 0 <= i && i < tableLen ==> table[i] == state(lin)[i]);
+  ensures subseq(vis, lin);
+  ensures res ==> state(vis)[witness_k] == v;
+  ensures !res ==> (forall i: int :: 0 <= i && i < tableLen ==> state(vis)[i] != v);
+{
+  var invoc: Invoc;
+  var old_lin, old_vis: SeqInvoc;
+  var k, tv: int;
+
+  vis := lin;  // Need to show forall j in hb :: j.vis subsetof vis
+  assert subseq(vis, lin);
+
+  k := 0;
+  while (k < tableLen)
+    invariant 0 <= k && k <= tableLen;
+    invariant subseq(vis, lin);
+    invariant (forall i: int :: 0 <= i && i < k ==> state(vis)[i] != v);
+    invariant (forall i: int :: 0 <= i && i < tableLen ==> table[i] == state(lin)[i]);
+  {
+    tv := table[k];
+
+    old_vis := vis;
+    vis := union(vis, restr(lin, k));
+    call lemma_union_restr(old_vis, vis, lin, k);
+    // tv == table[k] == state(lin)[k] == state(restr(lin, k))[k]
+    // == state(restr(vis, k))[k] == state(vis)[k]
+    assert tv == state(vis)[k];
+    // also, restr(lin, k) subseq lin ==> vis subseq lin
+    assert subseq(union(old_vis, restr(lin, k)), union(old_vis, lin));
+    assert subseq(union(old_vis, lin), union(lin, lin));
+    assert subseq(vis, lin);
+
+    if (tv == v) {
+      assert state(vis)[k] == v;
+      invoc := createInvoc(2, k, v);
+      old_lin := lin;
+      old_vis := vis;
+      lin := append(lin, invoc);
+      vis := append(vis, invoc);
+      call lemma_append_effect(old_lin, lin, invoc, 2, k, v);
+      call lemma_append_effect(old_vis, vis, invoc, 2, k, v);
+      witness_k := k;
+
+      res := true;
+      return;
+    }
+    // else tv != table[k] == state(lin)[k] == state(restr(lin, k))[k] == state(restr(vis, k))[k] == state(vis)[k]
+    k := k + 1;
+  }
+  invoc := createInvoc(2, k, v);
+  old_lin := lin;
+  old_vis := vis;
+  lin := append(lin, invoc);
+  vis := append(vis, invoc);
+  call lemma_append_effect(old_lin, lin, invoc, 2, k, v);
+  call lemma_append_effect(old_vis, vis, invoc, 2, k, v);
+
+  res := false;
+  return;
 }
